core/saved_prop.v
@@ -1,0 +1,88 @@
+From mathcomp Require Import ssreflect.
+From stdpp Require Import gmap.
+From iris.algebra Require Import agree auth gset gmap list reservation_map excl.
+From iris.algebra Require Import functions dfrac_agree.
+From iris.base_logic.lib Require Import invariants.
+From iris.heap_lang Require Import notation proofmode.
+From cryptis Require Import lib gmeta nown.
+From cryptis.core Require Import term comp_map minted.
+
+Definition savedPredR Σ A :=
+  dfrac_agreeR (oFunctor_apply (A -d> ▶ ∙) (iPropO Σ)).
+Definition savedPropR Σ :=
+  dfrac_agreeR (oFunctor_apply (▶ ∙) (iPropO Σ)).
+
+Class savedPredG Σ A := savedPred_inG : inG Σ (savedPredR Σ A).
+Class savedPropG Σ := savedProp_inG : inG Σ (savedPropR Σ).
+
+Definition savedPredΣ A :=
+  #[GFunctor (dfrac_agreeRF (A -d> ▶ ∙))].
+Definition savedPropΣ :=
+  #[GFunctor (dfrac_agreeRF (▶ ∙))].
+
+Global Existing Instance savedPred_inG.
+Global Existing Instance savedProp_inG.
+
+Global Instance subG_savedPredG Σ A : subG (savedPredΣ A) Σ → savedPredG Σ A.
+Proof. solve_inG. Qed.
+Global Instance subG_savedPropG Σ : subG savedPropΣ Σ → savedPropG Σ.
+Proof. solve_inG. Qed.
+
+Section SavedProp.
+
+Context `{Σ : gFunctors}.
+
+Implicit Types (dq : dfrac) (P Q : iProp Σ).
+
+Definition saved_prop (dq : dfrac) (P : iProp Σ) : savedPropR Σ :=
+  to_dfrac_agree dq (Next P).
+
+Lemma saved_prop_valid dq P : ✓ saved_prop dq P ↔ ✓ dq.
+Proof.
+rewrite /saved_prop /to_dfrac_agree pair_valid.
+by split=> [[] //|?]; split.
+Qed.
+
+Lemma saved_prop_validI dq P : ✓ saved_prop dq P ⊣⊢ (⌜✓ dq⌝ : iProp Σ).
+Proof. by rewrite /saved_prop dfrac_agree_validI. Qed.
+
+Lemma saved_prop_op_validI dq1 dq2 P Q :
+  ✓ (saved_prop dq1 P ⋅ saved_prop dq2 Q)
+  ⊣⊢ (⌜✓ (dq1 ⋅ dq2)⌝ ∧ ▷ (P ≡ Q) : iProp Σ).
+Proof.
+by rewrite /saved_prop dfrac_agree_validI_2 later_equivI.
+Qed.
+
+Context `{A : Type}.
+
+Implicit Types (φ ψ : A → iProp Σ).
+
+Definition saved_pred dq φ : savedPredR Σ A :=
+  to_dfrac_agree dq (Next ∘ φ : A -d> later (iProp Σ)).
+
+Lemma saved_pred_valid dq φ : ✓ saved_pred dq φ ↔ ✓ dq.
+Proof.
+rewrite /saved_pred /to_dfrac_agree pair_valid.
+by split=> [[] //|?]; split.
+Qed.
+
+Lemma saved_pred_validI dq φ : ✓ saved_pred dq φ ⊣⊢ (⌜✓ dq⌝ : iProp Σ).
+Proof. by rewrite /saved_pred dfrac_agree_validI. Qed.
+
+Lemma saved_pred_op_validI dq1 dq2 φ ψ :
+  ✓ (saved_pred dq1 φ ⋅ saved_pred dq2 ψ)
+  ⊣⊢ (⌜✓ (dq1 ⋅ dq2)⌝ ∧ □ (∀ x, ▷ (φ x ≡ ψ x)) : iProp Σ).
+Proof.
+rewrite /saved_pred dfrac_agree_validI_2.
+iSplit.
+- iIntros "[% #e]". iSplit => //.
+  iIntros "!> %x".
+  rewrite discrete_fun_equivI.
+  iSpecialize ("e" $! x).
+  by rewrite /= later_equivI.
+- iIntros "[% #e]". iSplit => //.
+  rewrite discrete_fun_equivI. iIntros "%x".
+  rewrite /= later_equivI. iApply "e".
+Qed.
+
+End SavedProp.
